Dafny/examples/simpleBenign/simpleBenignCommon.i.dfy
@@ -1,0 +1,51 @@
+include "BenignCode.s.dfy"
+include "../../LLVM/llvmREFACTOR.i.dfy"
+include "../../LLVM/types.dfy"
+include "../../Libraries/Seqs.s.dfy"
+
+module simpleBenignCommon{
+    import opened simpleBenignCode
+    import opened LLVM_defRE
+    import opened types
+    import opened Collections__Seqs_s
+
+
+    lemma unwrapPrintf(s:state,s':state, d:Data)// returns (b:behavior)
+        requires ValidState(s)
+        requires s' == evalInsRe(CALL(D(Void),printf_code(d).block),s)
+        requires ValidInstruction(s,CALL(D(Void),printf_code(d).block));
+        //ensures b == evalBlockRE(printf_code(d).block,s);
+        ensures StateNext(s,s')
+        ensures NextStep(s,s',Step.evalInsStep(CALL(D(Void),printf_code(d).block)));
+        {
+            reveal_behaviorOutput();
+            reveal_ValidBehavior();
+          //  b := [];
+            var subB := [s] + evalBlockRE(printf_code(d).block,s);
+            // assert |subB| == 2;
+            var step,remainder,subBehavior := unwrapBlockWitness(subB,printf_code(d).block,s); 
+            assert subB[0] == s;
+            assert NextStep(subB[0],subB[1],Step.evalInsStep(VISIBLE_OUT(Out(d))));
+            var s'' := s.(o := Out(d));
+            assert s'' == subB[1];
+            // assert s'' == s';
+            step,remainder,subBehavior := unwrapBlockWitness(subBehavior,remainder,last(step));
+            assert subB[1] == subB[2];  
+            assert NextStep(subB[1],subB[2],Step.stutterStep());
+            assert |subB| == 3;
+            assert ValidBehavior(subB);
+            assert ValidOperand(last(subB),D(Void));
+            //assert !D(Void).LV? && !D(Void).GV?;
+            assert validEvalIns(CALL(D(Void),printf_code(d).block),s,s');
+            assert s'.ok;
+            assert NextStep(s,s',Step.evalInsStep(CALL(D(Void),printf_code(d).block))) && StateNext(s,s');
+            assert evalBlockRE(printf_code(d).block,s) == [subB[1],subB[2]];
+            var x :=  evalInsRe(CALL(D(Void),printf_code(d).block),s);
+            assert s' == s.(o := SubOut(behaviorOutput([subB[1],subB[2]])));
+
+
+            // return [subB[1],subB[2]];
+
+
+        }
+}
