Dafny/examples/simpleBenign/simpleBenignisBenign.i.dfy
@@ -1,48 +1,107 @@
 include "BenignCode.s.dfy"
+include "simpleBenignCommon.i.dfy"
 include "../../LLVM/llvmREFACTOR.i.dfy"
 include "../../LLVM/types.dfy"
 include "../../Libraries/Seqs.s.dfy"
 
 module simpleBenignIsBenign{
     import opened simpleBenignCode
+    import opened simpleBenignCommon
     import opened LLVM_defRE
     import opened types
     import opened Collections__Seqs_s
 
 
-    lemma unwrapPatchBehaviors(s:state, input:operand) returns (b:behavior) 
+    lemma unwrapPatchSOIBehaviors(s:state, input:operand) returns (b:behavior) 
         requires ValidState(s);
-        requires validStartingState(s);
+        requires SOI_ASSIMPTIONS(s);
     {
-        var var_z := LV(" var_z ");
-        var var_cmp := LV(" var_cmp ");
-        var var_cmp1 := LV(" var_cmp1 ");
-        var var_add := LV(" var_add ");
+        reveal_ValidBehavior();
         var var_cmp2 := LV(" var_cmp2 ");
-        var var_0 := LV(" var_0 ");
+        var var_0:operand :| var_0.LV? && var_0.l in s.lvs && var_0.l == "var_0";
     
-        //reveal_BehaviorEvalsCode();
-        var c := benign_patch_code(input);
+        var c := benign_patch_SOI(s);
+        // var if_end := Block([
+        // Ins(ICMP(var_cmp2,ugt,4,var_0,D(Int(0,IntType(4,false))))),
+        // IfElse(true,if_then3().block,if_end4().block)]);
 
-        assert |c.block| == 3;
+        assert OperandContents(s,var_0).Int?;
+        assert OperandContents(s,var_0).val >= 2147483646;
+
+
+        assert |c.block| == 2;
 
         b := [s] + evalCodeRE(c,s);
+       
         var step,remainder,subBehavior := unwrapBlockWitness(b,c.block,s);
 
-        step,remainder,subBehavior := unwrapBlockWitness(subBehavior,remainder,last(step));
-            
-
-        //var var_z:LV := s.lvs["var_z"];
-
         assert b[0] == s;
-        assert "var_z" in s.lvs;
-        assert c.block[0] == Ins(ALLOCA(var_z,4));
-        //
-        assert b[1] == evalInsRe(ALLOCA(var_z,4),s);
-        assert ValidInstruction(s,ALLOCA(var_z,4));
+
+        assert ValidInstruction(s,ICMP(var_cmp2,ugt,4,var_0,D(Int(0,IntType(4,false)))));
+        assert NextStep(b[0],b[1],Step.evalInsStep(ICMP(var_cmp2,ugt,4,var_0,D(Int(0,IntType(4,false))))));
         assert StateNext(b[0],b[1]);
-        //assert ValidOperand(b[1],call);
 
+        assert step == [b[1]];
+        assert remainder == [IfElse(true,if_then3().block,if_end4().block)];
+        assert subBehavior == b[1..];
+        assert first(remainder).IfElse?;
+        step,remainder,subBehavior := unwrapBlockWitness(subBehavior,remainder,last(step));
 
+        assert step == [b[1]];
+        assert remainder == if_then3().block;
+        assert subBehavior == [b[1]] + evalBlockRE(remainder, b[1]); // no state change, just control flow
+
+        assert first(remainder).Ins?;
+        assert first(remainder).ins == CALL(D(Void),printf_code(global_str()).block);
+        step,remainder,subBehavior := unwrapBlockWitness(subBehavior,remainder,last(step));
+        
+
+        assert step == [b[2]];
+        assert b[2] == evalInsRe(CALL(D(Void),printf_code(global_str()).block),b[1]);
+        unwrapPrintf(b[1],b[2],global_str());
+        assert NextStep(b[1],b[2],Step.evalInsStep(CALL(D(Void),printf_code(global_str()).block)));
+        assert StateNext(b[1],b[2]); 
+        assert remainder == [if_end4()];
+        assert first(remainder).Block?;
+        assert subBehavior == [b[2]] + evalBlockRE(remainder, b[2]);
+
+        
+        step,remainder,subBehavior := unwrapBlockWitness(subBehavior,remainder,last(step));
+        assert step == [b[2]];
+        assert remainder == if_end4().block;
+        assert subBehavior == [b[2]] + evalBlockRE(remainder, b[2]); // no state change, just control flow
+
+        assert first(remainder).Ins?;
+        assert first(remainder).ins == CALL(D(Void),printf_code(global_str1()).block);
+
+        step,remainder,subBehavior := unwrapBlockWitness(subBehavior,remainder,last(step));
+        assert step == [b[3]];
+        assert b[3] == evalInsRe(CALL(D(Void),printf_code(global_str1()).block),b[2]);
+        unwrapPrintf(b[2],b[3],global_str1());
+        assert NextStep(b[2],b[3],Step.evalInsStep(CALL(D(Void),printf_code(global_str1()).block)));
+        assert StateNext(b[2],b[3]); 
+        assert remainder == [return_()];
+        assert first(remainder).Block?;
+        assert subBehavior == [b[3]] + evalBlockRE(remainder, b[3]);
+
+        step,remainder,subBehavior := unwrapBlockWitness(subBehavior,remainder,last(step));
+        assert step == [b[3]];
+        assert remainder == return_().block;
+        assert subBehavior == [b[3]] + evalBlockRE(remainder, b[3]);// no state change, just control flow
+
+        assert first(remainder).Ins?;
+        assert first(remainder).ins == RET(D(Void));
+        step,remainder,subBehavior := unwrapBlockWitness(subBehavior,remainder,last(step));
+        assert step == [b[4]];
+        assert b[4] == evalInsRe(RET(D(Void)),b[3]);
+        assert NextStep(b[3],b[4],Step.evalInsStep(RET(D(Void))));
+        assert StateNext(b[3],b[4]);
+
+        assert remainder == [];
+        assert subBehavior == [b[4]] + evalBlockRE(remainder, b[4]);
+        assert NextStep(b[4],b[5],Step.stutterStep());
+        // assert |b| == 7;
+        assert ValidBehavior(b);
+    
     }
 }
